Coq/Tools/total_order.v
@@ -1,0 +1,35 @@
+
+Require Import Relations.Relation_Definitions.
+
+Require Import relation_facts.
+Require Import preference.
+
+Definition total_order {T : Type} (R : relation T) : Prop :=
+  Relation_Definitions.reflexive T R /\ Relation_Definitions.transitive T R /\
+  Relation_Definitions.antisymmetric T R /\ total R.
+
+Definition TotalOrder (T : Type) : Type :=
+  { R : relation T | total_order R }.
+
+Lemma total_order_is_antisymmetric_preference {T : Type} (R : relation T) :
+  total_order R <-> (
+    preference_order R /\
+    Relation_Definitions.antisymmetric T R
+  ).
+Proof.
+  unfold total_order.
+  split.
+  {
+    intro.
+    unfold preference_order. tauto.
+  }
+  {
+    intro.
+    destruct H.
+    repeat split.
+    { apply preference_order_reflexive. exact H. }
+    { unfold preference_order in H. tauto. }
+    { exact H0. }
+    { unfold preference_order in H. tauto. }
+  }
+Qed.
